Cleaning up

proof/correctness/avx2/MLKEM_InnerPKE_avx2.ec
@@ -1960,24 +1960,51 @@ op lane_func_compress10(x : W16.t) : W10.t = truncate64_10 (
 
 op lane_polyvec_redcomp10(w : W16.t) : W10.t = lane_func_compress10 (lane_func_reduce w). 
 
-op lane(w : W16.t) : W16.t = w.
-op pcond (w: W16.t) = true.
-op pcond2 (w: W16.t) = w \ule W16.of_int (2*3329).
+op pcond_all (w: W16.t) = true.
+op pcond_reduced (w: W16.t) = w \ule W16.of_int (2*3329).
 
+lemma reduce_commutes x xr : xr = lane_func_reduce x => pcond_reduced xr.
+rewrite /lane_func_reduce /pcond_reduced. print Fq.SignedReductions.
+have := Fq.SignedReductions.BREDCp_corr (to_sint x) 26 _ _ _ _ _ _; rewrite ?qE /R //=.
++ admit. smt().
+  rewrite /BREDC.
+  admit.
+qed.
 
-lemma ref_reduce (_bp : W16.t Array768.t) : hoare [ AuxPolyVecCompress10.__poly_reduce : true ==> true].
+import BitEncoding.BitChunking.
+lemma ref_polyvec_reduce (_r : W16.t Array768.t) : hoare [ AuxPolyVecCompress10.__polyvec_reduce : r = _r ==> 
+  map lane_func_reduce
+      (map W16.bits2w (chunk 16 (flatten [flatten (map W16.w2bits (to_list _r))]))) =
+    map W16.bits2w (chunk 16 (flatten [flatten (map W16.w2bits (to_list res))]))].
 proc. 
 inline *.
-proc change ^while.5 : (sra_32 t0 (W32.of_int 26)).  admit.
-proc change ^while.9 : (W16_sub r (truncateu16 t0)). admit.
-unroll for ^while.
-wp 2816.
-bdep 16 16 [_bp] [rp] [rp]  lane_func_reduce pcond.
-admit. admit. 
+proc change 1 : (init_256_16 (fun i => r.[i])). admit.
+proc change ^while{1}.5 : (sra_32 t2 (W32.of_int 26)).  admit.
+proc change ^while{1}.9 : (W16_sub r0 (truncateu16 t2)). admit.
+proc change 5 : (init_768_16 (fun i => if 0 <= i < 256 then aux.[i] else r.[i])). admit.
+proc change 6 : (init_256_16 (fun i => r.[256+i])). admit.
+proc change ^while{2}.5 : (sra_32 t3 (W32.of_int 26)).  admit.
+proc change ^while{2}.9 : (W16_sub r1 (truncateu16 t3)). admit.
+proc change 10 : (init_768_16 (fun i => if 256 <= i < 512 then aux.[i-256] else r.[i])). admit.
+proc change 11 : (init_256_16 (fun i => r.[512+i])). admit.
+proc change ^while{3}.5 : (sra_32 t4 (W32.of_int 26)).  admit.
+proc change ^while{3}.9 : (W16_sub r2 (truncateu16 t4)). admit.
+proc change 15 : (init_768_16 (fun i => if 512 <= i < 768 then aux.[i-512] else r.[i])). admit.
+do 3!(unroll for ^while).
+cfold 2818.
+cfold 5637.
+cfold 8456.
+wp 8457.
+bdep 16 16 [_r] [r] [r]  lane_func_reduce pcond_all.
++ by move => *;rewrite /pcond_all -/predT;smt(all_predT).
+by smt().
 qed.
 
 
-lemma ref_compress (_bp : W16.t Array768.t) : hoare [ AuxPolyVecCompress10.__i_polyvec_compress_ref : true ==> true].
+lemma ref_polyvec_compress (_a : W16.t Array768.t) : hoare [ AuxPolyVecCompress10.__i_polyvec_compress_ref : 
+ a = _a /\ all pcond_reduced (map W16.bits2w (chunk 16 (flatten [flatten (map W16.w2bits (to_list _a))]))) ==>
+map lane_func_compress10 (map W16.bits2w (chunk 16 (flatten [flatten (map W16.w2bits (to_list _a))]))) =
+    map W10.bits2w (chunk 10 (flatten [flatten (map W8.w2bits (to_list res))]))].
 proc. 
 inline *. 
 proc change 1 : (init_960_8 (fun i => W8.zero)). admit.
@@ -2017,12 +2044,33 @@ cfold 3592.
 cfold 5387.
 cfold 5390.
 wp 14413.
-bdep 16 10 [_bp] [a] [rp]  lane_func_compress10 pcond2.
-admit. admit.
+bdep 16 10 [_a] [a] [rp]  lane_func_compress10 pcond_reduced. 
+by smt(). by smt().
 qed.
 
-op lane0(w : W16.t) = W16.zero.
-lemma avx_correctness (_bp : W16.t Array768.t) : hoare [ AuxPolyVecCompress10.avx2 : true ==> true].
+lemma ref_correctness (_bp : W16.t Array768.t) : hoare [ AuxPolyVecCompress10.ref :
+_bp = bp ==> 
+map lane_polyvec_redcomp10 (map W16.bits2w (chunk 16 (flatten [flatten (map W16.w2bits (to_list _bp))]))) =
+    map W10.bits2w (chunk 10 (flatten [flatten (map W8.w2bits (to_list res))]))
+].
+proof.
+proc.
+ecall (ref_polyvec_compress bp).
+ecall (ref_polyvec_reduce bp).
+auto => />. 
+move => inter Hreduce;split.
++ rewrite -Hreduce allP => x.
+  rewrite mapP => exm;elim exm => xrep.
+  rewrite mapP => exmm;elim exmm => xxrep.
+  by smt(reduce_commutes).
+move => preCompress fin.
+rewrite -Hreduce => <-. 
+by rewrite map_comp /=.
+qed.
+
+lemma avx_correctness (_bp : W16.t Array768.t) : hoare [ AuxPolyVecCompress10.avx2 : _bp = bp ==> 
+map lane_polyvec_redcomp10 (map W16.bits2w (chunk 16 (flatten [flatten (map W16.w2bits (to_list _bp))]))) =
+    map W10.bits2w (chunk 10 (flatten [flatten (map W8.w2bits (to_list res))]))].
 proof.
 proc.
 inline *.
@@ -2060,14 +2108,33 @@ cfold 183.
 cfold 365.
 cfold 547.
 wp 1807. 
-bdep 16 10 [_bp] [bp] [rp] lane_polyvec_redcomp10 pcond. 
-admit. admit.
+bdep 16 10 [_bp] [bp] [rp] lane_polyvec_redcomp10 pcond_all. 
++ by move => *;rewrite /pcond_all -/predT;smt(all_predT).
++ by smt().
 qed.
+
+lemma ref_correctness_p (_bp : W16.t Array768.t) : phoare [ AuxPolyVecCompress10.ref :
+_bp = bp ==> 
+map lane_polyvec_redcomp10 (map W16.bits2w (chunk 16 (flatten [flatten (map W16.w2bits (to_list _bp))]))) =
+    map W10.bits2w (chunk 10 (flatten [flatten (map W8.w2bits (to_list res))]))
+] = 1%r.
+admitted.
+
+lemma avx_correctness_p (_bp : W16.t Array768.t) : phoare [ AuxPolyVecCompress10.avx2 : _bp = bp ==> 
+map lane_polyvec_redcomp10 (map W16.bits2w (chunk 16 (flatten [flatten (map W16.w2bits (to_list _bp))]))) =
+    map W10.bits2w (chunk 10 (flatten [flatten (map W8.w2bits (to_list res))]))] = 1%r.
+admitted.
 
 (* MAP REDUCE GOAL *)
 lemma compress10_mr : 
   equiv [AuxPolyVecCompress10.avx2 ~ AuxPolyVecCompress10.ref : lift_array768 bp{1} = lift_array768 bp{2}==> ={res}].
-admitted.
+proc*.
+exlim bp{1}, bp{2} => _bp1 _bp2.
+call{1} (avx_correctness_p _bp1).
+call{2} (ref_correctness_p _bp2).
+auto => /> Hpre r1 Hr1 r2 Hr2.
+admit.
+qed.
 
 (*****************************************************************)
 
